Validity.v
@@ -1,6 +1,7 @@
 (**
 
-This file describes transformations of the layout of records and arrays.
+This file describes what it means for the different constructs in the
+language to be well-founded.
 
 Author: Ramon Fernandez I Mir and Arthur Charguéraud.
 
@@ -13,152 +14,166 @@ Require Export TLCbuffer Language.
 
 
 (* ---------------------------------------------------------------------- *)
-(** Validity of types *)
+(** Well-foundedness of types *)
 
-Inductive valid_typ (C:typdefctx) : typ -> Prop :=
-  | valid_typ_unit :
-      valid_typ C typ_unit
-  | valid_typ_int :
-      valid_typ C typ_int
-  | valid_typ_double :
-      valid_typ C typ_double
-  | valid_typ_bool :
-      valid_typ C typ_bool
-  | valid_typ_ptr : forall T,
-      valid_typ C T ->
-      valid_typ C (typ_ptr T)
-  | valid_typ_array : forall T os,
-      valid_typ C T ->
-      valid_typ C (typ_array T os)
-  | valid_typ_struct : forall Tfs,
+Inductive wf_typ (C:typdefctx) : typ -> Prop :=
+  | wf_typ_unit :
+      wf_typ C typ_unit
+  | wf_typ_int :
+      wf_typ C typ_int
+  | wf_typ_double :
+      wf_typ C typ_double
+  | wf_typ_bool :
+      wf_typ C typ_bool
+  | wf_typ_ptr : forall T,
+      wf_typ C T ->
+      wf_typ C (typ_ptr T)
+  | wf_typ_array : forall T os,
+      wf_typ C T ->
+      wf_typ C (typ_array T os)
+  | wf_typ_struct : forall Tfs,
       (forall f,
         f \indom Tfs ->
-        valid_typ C Tfs[f]) ->
-      valid_typ C (typ_struct Tfs)
-  | valid_typ_var : forall Tv,
+        wf_typ C Tfs[f]) ->
+      wf_typ C (typ_struct Tfs)
+  | wf_typ_var : forall Tv,
       Tv \indom C ->
-      valid_typ C C[Tv] ->
-      valid_typ C (typ_var Tv).
-
-Definition valid_phi (C:typdefctx) (φ:phi) : Prop :=
-  forall l,
-    l \indom φ ->
-    valid_typ C φ[l].
-
-Inductive valid_accesses (C:typdefctx) : accesses -> Prop :=
-  | valid_accesses_nil :
-      valid_accesses C nil 
-  | valid_accesses_cons_array : forall T i π,
-      valid_typ C T ->
-      valid_accesses C π ->
-      valid_accesses C ((access_array T i)::π)
-  | valid_accesses_cons_field : forall T f π,
-      valid_typ C T ->
-      valid_accesses C π ->
-      valid_accesses C ((access_field T f)::π).
+      wf_typ C C[Tv] ->
+      wf_typ C (typ_var Tv).
 
 
 (* ---------------------------------------------------------------------- *)
-(** Validity of values and terms *)
+(** Well-foundedness  of values and terms *)
 
-(* A value is valid if all of the types that appear in it are. *)
+(* A value is well-founded if all of the types that appear in it are. *)
 
-Inductive valid_val (C:typdefctx) : val -> Prop :=
-  | valid_val_uninitialized :
-      valid_val C val_uninitialized
-  | valid_val_unit :
-      valid_val C val_unit
-  | valid_val_bool : forall b,
-      valid_val C (val_bool b)
-  | valid_val_int : forall i,
-      valid_val C (val_int i)
-  | valid_val_double : forall d,
-      valid_val C (val_double d)
-  | valid_val_abstract_ptr : forall l π,
-      valid_accesses C π ->
-      valid_val C (val_abstract_ptr l π)
-  | valid_val_array : forall Ta a,
-      valid_typ C Ta ->
+Inductive wf_accesses (C:typdefctx) : accesses -> Prop :=
+  | wf_accesses_nil :
+      wf_accesses C nil 
+  | wf_accesses_cons_array : forall T i π,
+      wf_typ C T ->
+      wf_accesses C π ->
+      wf_accesses C ((access_array T i)::π)
+  | wf_accesses_cons_field : forall T f π,
+      wf_typ C T ->
+      wf_accesses C π ->
+      wf_accesses C ((access_field T f)::π).
+
+Inductive wf_val (C:typdefctx) : val -> Prop :=
+  | wf_val_error :
+      wf_val C val_error
+  | wf_val_uninitialized :
+      wf_val C val_uninitialized
+  | wf_val_unit :
+      wf_val C val_unit
+  | wf_val_bool : forall b,
+      wf_val C (val_bool b)
+  | wf_val_int : forall i,
+      wf_val C (val_int i)
+  | wf_val_double : forall d,
+      wf_val C (val_double d)
+  | wf_val_abstract_ptr : forall l π,
+      wf_accesses C π ->
+      wf_val C (val_abstract_ptr l π)
+  | wf_val_array : forall Ta a,
+      wf_typ C Ta ->
       (forall i,
         index a i ->
-        valid_val C a[i]) ->
-      valid_val C (val_array Ta a)
-  | valid_val_struct : forall Ts s,
-      valid_typ C Ts ->
+        wf_val C a[i]) ->
+      wf_val C (val_array Ta a)
+  | wf_val_struct : forall Ts s,
+      wf_typ C Ts ->
       (forall f,
         f \indom s ->
-        valid_val C s[f]) ->
-      valid_val C (val_struct Ts s).
+        wf_val C s[f]) ->
+      wf_val C (val_struct Ts s).
 
-(* A term is valid if all of the types that appear in it are. *)
+(* A term is well-founded if all of the types that appear in it are. *)
 
-Inductive valid_prim (C:typdefctx) : prim -> Prop :=
-  | valid_prim_binop : forall bop,
-      valid_prim C (prim_binop bop)
-  | valid_prim_get : forall T,
-      valid_typ C T ->
-      valid_prim C (prim_get T)
-  | valid_prim_set : forall T,
-      valid_typ C T ->
-      valid_prim C (prim_set T)
-  | valid_prim_new : forall T,
-      valid_typ C T ->
-      valid_prim C (prim_new T)
-  | valid_prim_new_array : forall T,
-      valid_typ C T ->
-      valid_prim C (prim_new_array T)
-  | valid_prim_struct_access : forall T f,
-      valid_typ C T ->
-      valid_prim C (prim_struct_access T f)
-  | valid_prim_array_access : forall T,
-      valid_typ C T ->
-      valid_prim C (prim_array_access T)
-  | valid_prim_struct_get : forall T f,
-      valid_typ C T ->
-      valid_prim C (prim_struct_get T f)
-  | valid_prim_array_get : forall T,
-      valid_typ C T ->
-      valid_prim C (prim_array_get T).
+Inductive wf_prim (C:typdefctx) : prim -> Prop :=
+  | wf_prim_binop : forall bop,
+      wf_prim C (prim_binop bop)
+  | wf_prim_get : forall T,
+      wf_typ C T ->
+      wf_prim C (prim_get T)
+  | wf_prim_set : forall T,
+      wf_typ C T ->
+      wf_prim C (prim_set T)
+  | wf_prim_new : forall T,
+      wf_typ C T ->
+      wf_prim C (prim_new T)
+  | wf_prim_new_array : forall T,
+      wf_typ C T ->
+      wf_prim C (prim_new_array T)
+  | wf_prim_struct_access : forall T f,
+      wf_typ C T ->
+      wf_prim C (prim_struct_access T f)
+  | wf_prim_array_access : forall T,
+      wf_typ C T ->
+      wf_prim C (prim_array_access T)
+  | wf_prim_struct_get : forall T f,
+      wf_typ C T ->
+      wf_prim C (prim_struct_get T f)
+  | wf_prim_array_get : forall T,
+      wf_typ C T ->
+      wf_prim C (prim_array_get T).
 
-Inductive valid_trm (C:typdefctx) : trm -> Prop :=
-  | valid_trm_val : forall v,
-      valid_val C v ->
-      valid_trm C (trm_val v)
-  | valid_trm_var : forall x,
-      valid_trm C (trm_var x)
-  | valid_trm_if : forall t0 t1 t2,
-      valid_trm C t0 ->
-      valid_trm C t1 ->
-      valid_trm C t2 ->
-      valid_trm C (trm_if t0 t1 t2)
-  | valid_trm_let : forall x t0 t1,
-      valid_trm C t0 ->
-      valid_trm C t1 ->
-      valid_trm C (trm_let x t0 t1)
-  | valid_trm_app_args_0 : forall op,
-      valid_prim C op ->
-      valid_trm C (trm_app op nil)
-  | valid_trm_app_args_1 : forall op t1,
-      valid_prim C op ->
-      valid_trm C t1 ->
-      valid_trm C (trm_app op (t1::nil))
-  | valid_trm_app_args_2 : forall op t1 t2,
-      valid_prim C op ->
-      valid_trm C t1 ->
-      valid_trm C t2 ->
-      valid_trm C (trm_app op (t1::t2::nil)).
+Inductive wf_trm (C:typdefctx) : trm -> Prop :=
+  | wf_trm_val : forall v,
+      wf_val C v ->
+      wf_trm C (trm_val v)
+  | wf_trm_var : forall x,
+      wf_trm C (trm_var x)
+  | wf_trm_if : forall t0 t1 t2,
+      wf_trm C t0 ->
+      wf_trm C t1 ->
+      wf_trm C t2 ->
+      wf_trm C (trm_if t0 t1 t2)
+  | wf_trm_let : forall x t0 t1,
+      wf_trm C t0 ->
+      wf_trm C t1 ->
+      wf_trm C (trm_let x t0 t1)
+  | wf_trm_app_args_0 : forall op,
+      wf_prim C op ->
+      wf_trm C (trm_app op nil)
+  | wf_trm_app_args_1 : forall op t1,
+      wf_prim C op ->
+      wf_trm C t1 ->
+      wf_trm C (trm_app op (t1::nil))
+  | wf_trm_app_args_2 : forall op t1 t2,
+      wf_prim C op ->
+      wf_trm C t1 ->
+      wf_trm C t2 ->
+      wf_trm C (trm_app op (t1::t2::nil)).
 
 
-(* Valid stack *)
+(* ---------------------------------------------------------------------- *)
+(** Well-foundedness of stack and state *)
 
-Definition valid_stack (C:typdefctx) (S:stack) : Prop :=
+(* Well-founded stack *)
+
+Definition wf_stack (C:typdefctx) (S:stack) : Prop :=
   forall x v,
     Ctx.lookup x S = Some v ->
-    valid_val C v.
+    wf_val C v.
 
-(* Valid state *)
+(* Well-founded state *)
 
-Definition valid_state (C:typdefctx) (m:state) : Prop :=
+Definition wf_state (C:typdefctx) (m:state) : Prop :=
   forall l,
     l \indom m ->
-    valid_val C m[l].
+    wf_val C m[l].
+
+(* Well-founded gamma *)
+
+Definition wf_gamma (C:typdefctx) (Γ:gamma) : Prop :=
+  forall x T,
+    Ctx.lookup x Γ = Some T ->
+    wf_typ C T.
+
+(* Well-founded phi *)
+
+Definition wf_phi (C:typdefctx) (φ:phi) : Prop :=
+  forall l,
+    l \indom φ ->
+    wf_typ C φ[l].
